Add a weight-preserving simplification during PropQuant computation

theories/iSL/PropQuantifiers.v
@@ -32,10 +32,38 @@ Section PropQuantDefinition.
 
 Local Notation "Δ '•' φ" := (cons φ Δ).
 
-(* solves the obligations of the following programs *)
-Obligation Tactic := intros; order_tac.
-
 Notation "□⁻¹ Γ" := (map open_box Γ) (at level 75).
+
+(** TODO: Experimental: weight_preserving simplifications *)
+
+Definition isimp (φ : form) : list form := [φ].
+Opaque isimp.
+
+Lemma env_order_refl_isimp φ: env_order_refl (isimp φ) [φ].
+Proof.
+Admitted.
+
+
+Lemma isim_vars {φ ψ x}: occurs_in x ψ -> ψ ∈ isimp φ -> occurs_in x φ.
+Proof.
+Admitted.
+
+Lemma isimp_complete_L (Γ : env) φ θ: Γ ⊎ list_to_set_disj (isimp φ) ⊢ θ -> Γ ⊎ {[φ]} ⊢ θ.
+Proof. Admitted.
+
+Ltac isimp_order := match goal with
+| |- ?Δ ++ isimp ?φ ≺ _ => eapply env_order_le_lt_trans;
+[apply env_order_refl_disj_union_compat ; [ isimp_order |apply (env_order_refl_isimp φ)]| 
+repeat rewrite <- Permutation_cons_append]
+| |- env_order_refl (_ ++ isimp _) _ =>
+apply env_order_refl_disj_union_compat; [ isimp_order|apply env_order_refl_isimp]
+| |- _ • _ ≺ _ => eapply env_order_le_lt_trans; [repeat apply env_order_eq_add; isimp_order|
+repeat rewrite <- Permutation_cons_append]
+| _ => right; reflexivity
+end.
+
+(* solves the obligations of the following programs *)
+Obligation Tactic := try solve[intros; order_tac; try isimp_order; order_tac].
 
 (** First, the implementation of the rules for calculating E. The names of the rules
   refer to the table in Pitts' paper. *)
@@ -52,23 +80,23 @@ match θ with
     if decide (p = q) then ⊤ (* default *)
     else q (* E1 modified *)
 (* E2 *)
-| δ₁ ∧ δ₂ => E ((Δ'•δ₁)•δ₂) _
+| δ₁ ∧ δ₂ => E ((Δ' ++ isimp δ₁) ++ isimp δ₂) _
 (* E3 *)
-| δ₁ ∨ δ₂ => E (Δ'•δ₁) _ ⊻ E (Δ' •δ₂) _
+| δ₁ ∨ δ₂ => E (Δ'•δ₁) _ ⊻ E (Δ'  ++ isimp δ₂) _
 | Var q → δ =>
-    if decide (Var q ∈ Δ) then E (Δ'•δ) _ (* E5 modified *)
+    if decide (Var q ∈ Δ) then E (Δ' ++ isimp δ) _ (* E5 modified *)
     else if decide (p = q) then ⊤
-    else q ⇢ E (Δ'•δ) _ (* E4 *)
+    else q ⇢ E (Δ' ++ isimp δ) _ (* E4 *)
 (* E6 *)
-| (δ₁ ∧ δ₂)→ δ₃ => E (Δ'•(δ₁ → (δ₂ → δ₃))) _
+| (δ₁ ∧ δ₂)→ δ₃ => E (Δ' ++ isimp (δ₁ → (δ₂ → δ₃))) _
 (* E7 *)
-| (δ₁ ∨ δ₂)→ δ₃ => E (Δ'•(δ₁ → δ₃)•(δ₂ → δ₃)) _
+| (δ₁ ∨ δ₂)→ δ₃ => E ((Δ' ++ isimp (δ₁ → δ₃)) ++ isimp (δ₂ → δ₃)) _
 (* E8 modified *)
 | ((δ₁→ δ₂)→ δ₃) =>
-  (E (Δ'•(δ₂ → δ₃) • δ₁) _⇢ A (Δ'•(δ₂ → δ₃) • δ₁, δ₂) _) ⇢ E (Δ'•δ₃) _
+  (E ((Δ' ++ isimp (δ₂ → δ₃)) ++ isimp  δ₁) _⇢ A ((Δ' ++ isimp (δ₂ → δ₃)) ++ isimp  δ₁, δ₂) _) ⇢ E (Δ' ++ isimp δ₃) _
 | Bot → _ => ⊤
-| □ φ => □(E ((□⁻¹ Δ') • φ ) _) (* very redundant ; identical for each box *)
-| (□δ1 → δ2) =>  (□(E((□⁻¹ Δ') • δ2 • □δ1) _ ⇢ A((□⁻¹ Δ') • δ2 • □δ1, δ1) _)) ⇢ E(Δ' • δ2) _
+| □ φ => □(E ((□⁻¹ Δ') ++ isimp  φ ) _) (* very redundant ; identical for each box *)
+| (□δ1 → δ2) =>  (□(E(((□⁻¹ Δ') ++ isimp  δ2) ++ isimp  (□δ1)) _ ⇢ A(((□⁻¹ Δ') ++ isimp  δ2) ++ isimp  (□δ1), δ1) _)) ⇢ E(Δ'  ++ isimp  δ2) _
 end.
 
 
@@ -89,29 +117,31 @@ match θ with
       else ⊥
     else ⊥ (* A1 modified : A (Δ', ϕ) can be removed *)
 (* A2 *)
-| δ₁ ∧ δ₂ => A ((Δ'•δ₁)•δ₂, ϕ) _
+| δ₁ ∧ δ₂ => A ((Δ' ++ isimp δ₁) ++ isimp δ₂, ϕ) _
 (* A3 *)
 | δ₁ ∨ δ₂ =>
-      (E (Δ'•δ₁) _ ⇢ A (Δ'•δ₁, ϕ) _)
-  ⊼ (E (Δ'•δ₂) _ ⇢ A (Δ'•δ₂, ϕ) _)
+      (E (Δ' ++ isimp δ₁) _ ⇢ A (Δ' ++ isimp δ₁, ϕ) _)
+  ⊼ (E (Δ' ++ isimp δ₂) _ ⇢ A (Δ' ++ isimp δ₂, ϕ) _)
 | Var q → δ =>
     if decide (Var q ∈ Δ) then A (Δ'•δ, ϕ) _ (* A5 modified *)
     else if decide (p = q) then ⊥
-    else q ⊼ A (Δ'•δ, ϕ) _ (* A4 *)
+    else q ⊼ A (Δ' ++ isimp δ, ϕ) _ (* A4 *)
 (* A6 *)
 | (δ₁ ∧ δ₂)→ δ₃ =>
-  A (Δ'•(δ₁ → (δ₂ → δ₃)), ϕ) _
+  A (Δ' ++ isimp (δ₁ → (δ₂ → δ₃)), ϕ) _
 (* A7 *)
 | (δ₁ ∨ δ₂)→ δ₃ =>
-  A ((Δ'•(δ₁ → δ₃))•(δ₂ → δ₃), ϕ) _
+  A ((Δ' ++ isimp (δ₁ → δ₃)) ++ isimp (δ₂ → δ₃), ϕ) _
 (* A8 modified*)
 | ((δ₁→ δ₂)→ δ₃) =>
-  (E (Δ'•(δ₂ → δ₃) • δ₁) _ ⇢ A (Δ'•(δ₂ → δ₃) • δ₁, δ₂) _)
-  ⊼ A (Δ'•δ₃, ϕ) _
+  (E ((Δ'  ++ isimp (δ₂ → δ₃)) ++ isimp  δ₁) _ ⇢ A ((Δ'  ++ isimp (δ₂ → δ₃) )++ isimp  δ₁, δ₂) _)
+  ⊼ A (Δ' ++ isimp δ₃, ϕ) _
 | Bot => ⊥
 | Bot → _ => ⊥
 | □δ => ⊥
-| ((□δ1) → δ2) => (□(E((□⁻¹ Δ')• δ2 • □δ1) _  ⇢ A((□⁻¹ Δ')• δ2 • □δ1, δ1) _)) ∧ A(Δ' • δ2, ϕ) _
+| ((□δ1) → δ2) => (□(E(((□⁻¹ Δ') ++ isimp  δ2 ) ++ isimp  (□δ1)) _  
+                              ⇢ A(((□⁻¹ Δ') ++ isimp  δ2 ) ++ isimp  (□δ1), δ1) _))
+                          ∧ A(Δ' ++ isimp δ2, ϕ) _
 (* using ⊼ here breaks congruence *)
 end.
 
@@ -137,6 +167,7 @@ match ϕ with
 | Bot => ⊥
 | □δ => □((E ((□⁻¹ Δ) • □δ, δ) _) ⇢ A((□⁻¹ Δ) • □δ, δ) _)
 end.
+(* TODO: use isimp here too? *)
 
 Obligation Tactic := intros; order_tac.
 Program Fixpoint EA (pe : list form * form) {wf pointed_env_order pe} :=
@@ -262,6 +293,8 @@ try match goal with
 | H : occurs_in _ (?a ⇢ ?b) |- _ => apply occurs_in_make_impl in H
 | H : occurs_in _ (?a ⊻ ?b) |- _ => apply occurs_in_make_disj in H
 | H : occurs_in _ (?a ⊼ ?b) |- _ => apply occurs_in_make_conj in H
+|H1 : ?x0 ∈ (?Δ ++ _), H2 : occurs_in ?x ?x0 |- _ => repeat rewrite elem_of_app in H1
+|H1 : ?x0 ∈ (isimp _), H2 : occurs_in ?x ?x0 |- _ => apply (isim_vars H2) in H1
 |H1 : ?x0 ∈ (⊗ ?Δ), H2 : occurs_in ?x ?x0 |- _ =>
       apply (occurs_in_open_boxes _ _ _ H2) in H1
 |H1 : ?x0 ∈ (map open_box ?Δ), H2 : occurs_in ?x ?x0 |- _ =>
@@ -378,7 +411,14 @@ rewrite (proper_Provable _ _ (equiv_disj_union_compat_r (equiv_disj_union_compat
   + subst. case_decide; subst; auto with proof.
   + exch 0...
 - constructor 2.
-- simpl; exch 0. apply AndL. exch 1; exch 0. do 2 l_tac...
+- simpl; exch 0. apply AndL.
+(* requires a specific lemma using isimp_complete_L, equiv_assoc and list_to_set_disj_app *)
+assert((list_to_set_disj (((rm (θ1 ∧ θ2) Δ) ++ isimp θ1) ++ isimp θ2)
+ • (EA0 ((rm (θ1 ∧ θ2) Δ ++ isimp θ1) ++ isimp θ2, ϕ)
+      (a_rule_env_obligation_1 Δ ϕ (θ1 ∧ θ2) Hin θ1 θ2 eq_refl)).2) ⊢ ϕ).
+      
+auto with proof.
+ exch 1; exch 0. do 2 l_tac...
 - apply make_conj_sound_L.
   exch 0. apply OrL; exch 0.
   + apply AndL. apply make_impl_sound_L. exch 0. apply make_impl_sound_L.
